---
id: W283ieuL
vimeo: 454396130
---

Below is a sketch of
$$
y = \frac{1}{(x-1)(x+2)}
$$

![](/img/learn/enlargement-1.png)

Hence, sketch
$$
y = \frac{1}{2(2x-1)(x+1)}
$$

---

Let
$$
f(x) = \frac{1}{(x-1)(x+2)}
$$
be the original function, which is sketched for us.

Write the new function as
$$
\frac{1}{2(2x-1)(x+2)} = \frac{1}{(2x-1)(2x+2)}
$$
(we have put the $2$ into the second bracket).

---

Based on the hint above, $x$ has been replaced with $2x,$ so we have to sketch
$$
y = f(2x)
$$
which is an enlargement, scale factor $\frac{1}{2}$, parallel to the $x$ axis.
