---
title: Differentiating $e^{kx}$
id: rFiX7MBv
vimeo: 111
problems:
  - XjCFHeZA
  - TOUueUCF
  - R2OM3SNg
  - dryRDLMf
  - aHkEf2UE
  - cizJaH62
  # - gmXxQpGJ
  # - tptvbj1u
  # - IqzjhILs
  # - XO1UV6ha
---

## Differentiating $e^x$

The number $e$ is, as we have mentioned before, a very important number. It is important because
$$
y = e^x \, \Rightarrow \frac{dy}{dx} = e^x
$$
We sometimes say that $e^x$ *differentiates to itself.*

This means that the gradient of the curve $y = e^x$ is equal to $e^x,$ as you can see by moving the below point around:

<geogebra id="wfgvddxx"></geogebra>

## Differentiating $e^{kx}$

We can also differentiate functions of the form
$$
y = e^{kx}
$$
where $k$ is some number.

If
$$
f(x) = e^x
$$
then
$$
f(kx) = e^{kx}
$$
is an enlargement in the $x$ direction of scale factor $\frac{1}{k}.$ This makes the gradient *steeper* by a scale factor of $k,$ as you can see below:

<geogebra id="ndgvgscj"></geogebra>

This suggests that
$$
y = e^{kx} \, \Rightarrow \frac{dy}{dx} = ke^{kx}
$$
We're going to assume this is true for now - we'll be able to prove in a couple of chapters' time when we study the chain rule.

---

Let
$$
f(x) = \left( e^{\frac{x}{2}} - 3e^{-x} \right)e^{x}
$$
and
$$
g(x) = \frac{e^{x} + 2e^{3x}}{e^{5x}}
$$
Find $f'(x)$ and $g'(x)$
